\lecture{16}{2022-02-23}{}

\begin{defn}{\(p\)-norm}{}
	Given \(f \in L^p(\mathbb{R})\), define \[
		\|f\|_p = \left( \int_{-\infty}^\infty |f(x)|^p\,dx \right)^{1/p}.
	\] 
\end{defn}

\section{Convex Functions}

\begin{defn}{Convex Function}{}
	Given an interval \(A \subset \mathbb{R}\), a function \(f \colon A \to \mathbb{R}\) is \emph{convex} if, and only if, \[
		f(\lambda x + (1 - \lambda) y) \leq \lambda f(x) + (1-\lambda) f(y),
	\] 
	for all \(x, y \in A\) and \(\lambda \in [0, 1]\).
\end{defn}

\begin{exmp}{}{}
	The functions \(f\colon \mathbb{R} \to \mathbb{R}\) and \(g \colon [0, +\infty) \to \mathbb{R}\) defined by \(f(x) = |x|\) and \(g(x) = x^p\), for \(p > 1\), are convex functions.
\end{exmp}

\begin{thm}{}{}
	Given an interval \(A\), and a convex function \(f \colon A \to \mathbb{R}\), if \(f(A)\) is an interval and \(g \colon f(A) \to \mathbb{R}\) is a convex function, then \(g \circ f\) is convex on \(A\).
\end{thm}

\begin{prop}{}{}
	The \(p\)-norm indeed satisfies the triangle inequality. In other words, for all \(f, g \in L^p(\mathbb{R})\), \[
		\left( \int_{-\infty}^\infty |f(x) + g(x)|^p\,dx \right)^{1/p} \leq
		\left( \int_{-\infty}^\infty |f(x)|^p\,dx \right)^{1/p} +
		\left( \int_{-\infty}^\infty |g(x)|^p\,dx \right)^{1/p}.
	\] 
\end{prop}

\section{\texorpdfstring{$L^2(\mathbb{R})$}{L\texttwosuperior(R)} is special}

\begin{thm}{}{}
	If \(f, g \in L^2(\mathbb{R})\), then \(fg \in L^1(\mathbb{R})\), with \[
		\int_{-\infty}^\infty |f(x)g(x)|\,dx
		\leq \|f\|_2 \|g\|_2.
	\] 
\end{thm}

\begin{defn}{Inner product in \(L^2(\mathbb{R})\)}{}
	Given \(f, g \in L^2(\mathbb{R})\), we define their inner product by \[
		\langle f, g \rangle = \int_{-\infty}^\infty f(x)g(x)\,dx.
	\] 
\end{defn}

\begin{prop}{}{}
	For all \(f, g, h \in L^2(\mathbb{R})\) and \(c \in \mathbb{R}\), 
	\begin{enumerate}
		\item \(\langle f, g \rangle = \langle g, f \rangle\).
		\item \(\langle f, f \rangle \geq 0\), and the equality holds if, and only if, \(f = 0\).
		\item \(\langle f + g, h \rangle = \langle f, h \rangle + \langle g, h \rangle\).
		\item \(\langle cf, g \rangle = c\langle f, g \rangle\).
	\end{enumerate}
\end{prop}
